more examples

thys/Untyped_Lambda_Calculus/LC_Parallel_Beta.thy
@@ -4,227 +4,61 @@ theory LC_Parallel_Beta
 imports LC "Binders.Generic_Barendregt_Enhanced_Rule_Induction" "Prelim.Curry_LFP" 
 begin
 
-(* INSTANTIATING THE ABSTRACT SETTING: *)
+fun Tperm where "Tperm f (a,b) = ((rrename f a,rrename f b))"
+fun Tsupp where "Tsupp (a,b) = FFVars a \<union> FFVars b"
 
-(* *)
+lemma fresh: "\<exists>xx. xx \<notin> Tsupp (t :: trm \<times> trm)"
+  using Tsupp.simps[of "fst t" "snd t"] unfolding prod.collapse
+  by (metis (no_types, lifting) exists_var finite_iff_le_card_var term.Un_bound term.set_bd_UNIV)
 
-inductive pstep :: "trm \<Rightarrow> trm \<Rightarrow> bool" where
+binder_inductive pstep :: "trm \<Rightarrow> trm \<Rightarrow> bool" where
   Refl: "pstep e e"
 | App: "pstep e1 e1' \<Longrightarrow> pstep e2 e2' \<Longrightarrow> pstep (App e1 e2) (App e1' e2')"
-| Xi: "pstep e e' \<Longrightarrow> pstep (Lam x e) (Lam x e')"
-| PBeta: "pstep e1 e1' \<Longrightarrow> pstep e2 e2' \<Longrightarrow> pstep (App (Lam x e1) e2) (tvsubst (Var(x:=e2')) e1')"
-
-thm pstep_def
-
-(* xx fresh \<Longrightarrow> tvsubst (Var(x:=e2')) e1' = tvsubst (Var(xx:=e2')) e1'[xx\<and>x]  *)
-
-(* INSTANTIATING THE LSNominalSet LOCALE: *)
-
-type_synonym T = "trm \<times> trm"
-
-(* type_synonym V = "var list" (* in this case, could have also taken to be 'a option; 
-and the most uniform approach would have been 'a + unit + 'a + 'a *) *)
-
-
-definition Tperm :: "(var \<Rightarrow> var) \<Rightarrow> T \<Rightarrow> T" where 
-"Tperm f \<equiv> map_prod (rrename_term f) (rrename_term f)"
-
-fun Tsupp :: "T \<Rightarrow> var set" where 
-"Tsupp (e1,e2) = FFVars_term e1 \<union> FFVars_term e2"
-
-(* definition Vmap :: "(var \<Rightarrow> var) \<Rightarrow> V \<Rightarrow> V" where 
-"Vmap \<equiv> map"
-
-fun Vfvars :: "V \<Rightarrow> var set" where 
-"Vfvars v = set v"  *)
-
-interpretation LSNominalSet where 
-Tperm = Tperm and Tsupp = Tsupp
-(* and Vmap = Vmap and Vfvars = Vfvars *)
-apply standard unfolding isPerm_def Tperm_def  
-  using small_Un small_def term.card_of_FFVars_bounds
-  apply (auto simp: term.rrename_id0s map_prod.comp term.rrename_comp0s infinite_UNIV)
-  using var_sum_class.Un_bound by blast
-
-definition G :: "var set \<Rightarrow> (T \<Rightarrow> bool) \<Rightarrow> T \<Rightarrow> bool"
-where
-"G \<equiv> \<lambda>B R t.  
-         (B = {} \<and> fst t = snd t)
-         \<or>
-         (\<exists>e1 e1' e2 e2'. B = {}  \<and> fst t = App e1 e2 \<and> snd t = App e1' e2' \<and> 
-                          R (e1,e1') \<and> R (e2,e2')) 
-         \<or>
-         (\<exists>x e e'. B = {x} \<and> fst t = Lam x e \<and> snd t = Lam x e' \<and> R (e,e'))
-         \<or>
-         (\<exists>x e1 e1' e2 e2'. B = {x}  \<and> fst t = App (Lam x e1) e2 \<and> snd t = tvsubst (Var(x := e2')) e1' \<and> 
-            R (e1,e1') \<and> R (e2,e2'))"
-
-
-(* VERIFYING THE HYPOTHESES FOR BARENDREGT-ENHANCED INDUCTION: *)
-
-lemma G_mono: "R \<le> R' \<Longrightarrow> small B \<Longrightarrow> G B R t \<Longrightarrow> G B R' t"
-unfolding G_def by fastforce
-
-(* NB: Everything is passed \<sigma>-renamed as witnesses to exI *)
-lemma G_equiv: "isPerm \<sigma> \<Longrightarrow> small B \<Longrightarrow> G B R t \<Longrightarrow> G (image \<sigma> B) (\<lambda>t'. R (Tperm (inv \<sigma>) t')) (Tperm \<sigma> t)"
-  unfolding G_def
-  by (elim disj_forward exE; cases t)
-    (auto simp: Tperm_def isPerm_def
+| Xi: "pstep e e' \<Longrightarrow> pstep (Lam x e) (Lam x e')" binds "{x}"
+| PBeta: "pstep e1 e1' \<Longrightarrow> pstep e2 e2' \<Longrightarrow> pstep (App (Lam x e1) e2) (tvsubst (Var(x:=e2')) e1')" binds "{x}"
+where perm: Tperm supp: Tsupp
+         apply (auto simp: o_def split_beta term.rrename_comps fun_eq_iff isPerm_def
+           small_def term.card_of_FFVars_bounds term.Un_bound) [5]
+  subgoal for R R' B t
+    by fastforce
+  subgoal for \<sigma> R B t
+    unfolding split_beta
+    by (elim disj_forward exE; cases t)
+      (auto simp: isPerm_def
          term.rrename_comps rrename_tvsubst_comp
          | ((rule exI[of _ "\<sigma> _"] exI)+, (rule conjI)?, rule refl)
          | ((rule exI[of _ "\<sigma> _"])+; auto))+
-(*
-  unfolding G_def apply(elim disjE)
-  subgoal apply(rule disjI4_1)
-  subgoal  
-  apply(cases t) unfolding isPerm_def small_def Tperm_def  
-  by simp . 
-  (* *)
-  subgoal apply(rule disjI4_2)
-  subgoal apply(elim exE) subgoal for e1 e1' e2 e2'
-  apply(rule exI[of _ "rrename_term \<sigma> e1"]) apply(rule exI[of _ "rrename_term \<sigma> e1'"]) 
-  apply(rule exI[of _ "rrename_term \<sigma> e2"]) apply(rule exI[of _ "rrename_term \<sigma> e2'"])
-  apply(cases t) unfolding isPerm_def small_def Tperm_def 
-  by (simp add: term.rrename_comps) . . 
-  (* *)
-  subgoal apply(rule disjI4_3)
-  subgoal apply(elim exE) subgoal for x e e'
-  apply(rule exI[of _ "\<sigma> x"])
-  apply(rule exI[of _ "rrename_term \<sigma> e"]) apply(rule exI[of _ "rrename_term \<sigma> e'"]) 
-  apply(cases t) unfolding isPerm_def small_def Tperm_def  
-  by (simp add: term.rrename_comps) . . 
-  (* *)
-  subgoal apply(rule disjI4_4)
-  subgoal apply(elim exE) subgoal for x e1 e1' e2 e2'
-  apply(rule exI[of _ "\<sigma> x"])
-  apply(rule exI[of _ "rrename_term \<sigma> e1"]) apply(rule exI[of _ "rrename_term \<sigma> e1'"]) 
-  apply(rule exI[of _ "rrename_term \<sigma> e2"]) apply(rule exI[of _ "rrename_term \<sigma> e2'"]) 
-  apply(cases t) unfolding isPerm_def small_def Tperm_def 
-  apply (simp add: term.rrename_comps) apply(subst rrename_tvsubst_comp) by auto
- . . . 
-*)
-  
+  subgoal premises prems for R B t
+    using fresh[of t] prems(2-) unfolding
+      (**)isPerm_def conj_assoc[symmetric] split_beta
+    unfolding ex_push_inwards conj_disj_distribL ex_disj_distrib
+    apply (elim disj_forward exE; simp)
+     apply (((rule exI, rule conjI[rotated], assumption) |
+          (((rule exI conjI)+)?, rule Lam_refresh tvsubst_refresh) |
+          (cases t; auto split: if_splits))+) []
+    subgoal for xx e1 e1' e2 e2' x
+    apply (subst (2 3) ex_comm; simp)
+      apply (erule exE conjE)+
+      apply (erule thin_rl[of "R (e1, e1')"])
+      apply (erule thin_rl[of "R (e2, e2')"])
+    apply (rule exI)
+    apply (rule exI[of _ "{xx}"])
+    apply (rule conjI)
+    apply (rule exI)
+       apply (rule conjI[OF refl])
+       apply (rule conjI[OF Lam_refresh])
+      apply (cases t; simp)
+       apply (rule exI)+
+       apply (rule conjI[rotated])+
+         apply assumption
+        apply blast
+      apply (cases t)
+       apply (fastforce intro!: tvsubst_refresh)
+      apply simp
+      done
+    done
+  done
 
-lemma fresh: "\<exists>xx. xx \<notin> Tsupp t"  
-by (metis Lam_avoid Tsupp.elims term.card_of_FFVars_bounds term.set(2))
-
-(* NB: The entities affected by variables are passed as witnesses to exI 
-with x and (the fresh) xx swapped, whereas the non-affected ones are passed 
-as they are. 
-*)
-lemma G_refresh: 
-"(\<forall>\<sigma> t. isPerm \<sigma> \<and> R t \<longrightarrow> R (Tperm \<sigma> t)) \<Longrightarrow> small B \<Longrightarrow> G B R t \<Longrightarrow> 
- \<exists>C. small C \<and> C \<inter> Tsupp t = {} \<and> G C R t"
-  using fresh[of t] unfolding G_def Tperm_def
-(**)isPerm_def conj_assoc[symmetric]
-  unfolding ex_push_inwards conj_disj_distribL ex_disj_distrib
-  apply (elim disj_forward exE; simp)
-  apply (((rule exI, rule conjI[rotated], assumption) |
-    (((rule exI conjI)+)?, rule Lam_refresh tvsubst_refresh) |
-    (cases t; auto split: if_splits))+) []
-  apply (((rule exI, rule conjI[rotated], assumption) |
-    (((rule exI conjI)+)?, rule Lam_refresh tvsubst_refresh) |
-    (cases t; auto split: if_splits)))
-  apply (((rule exI, rule conjI[rotated], assumption) |
-    (((rule exI conjI)+)?, rule Lam_refresh tvsubst_refresh) |
-    (cases t; auto split: if_splits)))
-  apply (((rule exI, rule conjI[rotated], assumption) |
-    (((rule exI conjI)+)?, rule Lam_refresh tvsubst_refresh) |
-    (cases t; auto split: if_splits)))
-  apply (((rule exI, rule conjI[rotated], assumption) |
-    (((rule exI conjI)+)?, rule Lam_refresh tvsubst_refresh) |
-    (cases t; auto split: if_splits)))
-  apply (cases t; simp split: if_splits) []
-  apply (metis insertI1)
-  apply (((rule exI, rule conjI[rotated], assumption) |
-    (((rule exI conjI)+)?, rule Lam_refresh tvsubst_refresh) |
-    (cases t; auto split: if_splits)))
-(*
-using fresh[of t] unfolding G_def Tperm_def apply safe
-  subgoal for xx
-  apply(rule exI[of _ "{}"])    
-  apply(intro conjI)
-    subgoal by simp 
-    subgoal by simp 
-    subgoal apply(rule disjI4_1) by simp . 
-  (* *)
-  subgoal for xx e1 e1' e2 e2'
-  apply(rule exI[of _ "{}"])  
-  apply(intro conjI)
-    subgoal by simp
-    subgoal unfolding isPerm_def small_def by auto 
-    subgoal apply(rule disjI4_2) 
-    apply(rule exI[of _ "e1"]) 
-    apply(rule exI[of _ "e1'"])
-    apply(rule exI[of _ "e2"]) 
-    apply(rule exI[of _ "e2'"])
-    apply(cases t)  apply simp . .
-  (* *)
-  subgoal for xx x e e'
-  apply(rule exI[of _ "{xx}"])  
-  apply(intro conjI)
-    subgoal by simp
-    subgoal unfolding isPerm_def small_def by auto 
-    subgoal apply(rule disjI4_3) 
-    apply(rule exI[of _ "xx"]) 
-    apply(rule exI[of _ "rrename_term (id(x:=xx,xx:=x)) e"])
-    apply(rule exI[of _ "rrename_term (id(x:=xx,xx:=x)) e'"])
-    apply(cases t)  apply simp apply(intro conjI)
-      subgoal apply(subst Lam_rrename[of "id(x:=xx,xx:=x)"]) by auto
-      subgoal apply(subst Lam_rrename[of "id(x:=xx,xx:=x)"]) by auto
-      subgoal by (metis supp_swap_bound Prelim.bij_swap isPerm_def) . . 
-  (* *)
-  subgoal for xx x e1 e1' e2 e2'
-  apply(rule exI[of _ "{xx}"])  
-  apply(intro conjI)
-    subgoal by simp
-    subgoal unfolding isPerm_def small_def by auto 
-    subgoal apply(rule disjI4_4)
-    apply(rule exI[of _ "xx"]) 
-    apply(rule exI[of _ "rrename_term (id(x:=xx,xx:=x)) e1"])
-    apply(rule exI[of _ "rrename_term (id(x:=xx,xx:=x)) e1'"])
-    apply(rule exI[of _ "e2"])
-    apply(rule exI[of _ "e2'"])
-    apply(cases t)  apply simp apply(intro conjI)
-      subgoal apply(subst Lam_rrename[of "id(x:=xx,xx:=x)"]) by auto
-      subgoal apply(subst tvsubst_Var_rrename) 
-      apply (auto split: if_splits)   
-      by blast
-      subgoal by (metis supp_swap_bound Prelim.bij_swap isPerm_def) . .*) . 
-  (* *)
-
-
-(* FINALLY, INTERPRETING THE Induct LOCALE: *)
-
-interpretation Pstep: Induct where
-Tperm = Tperm and Tsupp = Tsupp and G = G
-apply standard 
-  using G_mono G_equiv G_refresh by auto
-
-(* *)
-
-lemma pstep_I: "pstep t1 t2 = Pstep.I (t1,t2)" 
-unfolding pstep_def Pstep.I_def lfp_curry2 apply(rule arg_cong2[of _ _ _ _ lfp], simp_all)
-unfolding fun_eq_iff G_def apply clarify
-subgoal for R tt1 tt2 apply(rule iffI)
-  subgoal apply(elim disjE exE)
-    \<^cancel>\<open>Refl: \<close>
-    subgoal apply(rule exI[of _ "{}"], rule conjI, simp) apply(rule disjI4_1) by auto
-    \<^cancel>\<open>App: \<close>
-    subgoal apply(rule exI[of _ "{}"], rule conjI, simp)  apply(rule disjI4_2) by auto
-    \<^cancel>\<open>Xi: \<close>
-    subgoal for e e' x apply(rule exI[of _ "{x}"], rule conjI, simp)  apply(rule disjI4_3) by auto
-    \<^cancel>\<open>PBeta: \<close>
-    subgoal for e1 e1' e2 e2' x apply(rule exI[of _ "{x}"], rule conjI, simp) apply(rule disjI4_4) by auto .
-  subgoal apply(elim conjE disjE exE)
-    \<^cancel>\<open>Refl: \<close>
-    subgoal apply(rule disjI4_1) by auto
-    \<^cancel>\<open>App: \<close>
-    subgoal apply(rule disjI4_2) by auto
-    \<^cancel>\<open>Xi: \<close>
-    subgoal apply(rule disjI4_3) by auto
-    \<^cancel>\<open>PBeta: \<close>
-    subgoal apply(rule disjI4_4) by auto . . .
 
 (* FROM ABSTRACT BACK TO CONCRETE: *)
 thm pstep.induct[no_vars]
@@ -246,25 +80,25 @@ and PBeta: "\<And>x e1 e1' e2 e2' p.
   pstep e2 e2' \<Longrightarrow> (\<forall>p'. R p' e2 e2') \<Longrightarrow> 
   R p (App (Lam x e1) e2) (tvsubst (VVr(x := e2')) e1')"
 shows "R p t1 t2"
-unfolding pstep_I
+unfolding pstep.alt_def
 apply(subgoal_tac "case (t1,t2) of (t1, t2) \<Rightarrow> R p t1 t2")
   subgoal by simp
-  subgoal using par st apply(elim Pstep.strong_induct[where R = "\<lambda>p (t1,t2). R p t1 t2"])
-    subgoal unfolding pstep_I by simp
-    subgoal for p B t apply(subst (asm) G_def) 
-    unfolding pstep_I[symmetric] apply(elim disjE exE)
+  subgoal using par st apply(elim pstep.strong_induct[where R = "\<lambda>p (t1,t2). R p t1 t2"])
+    subgoal unfolding pstep.alt_def by simp
+    subgoal for p B t
+    unfolding pstep.alt_def[symmetric] apply(elim disjE exE case_prodE)
       subgoal using Refl by auto
       subgoal using App by auto  
       subgoal using Xi by auto
-      subgoal for x e1 e1' e2 e2' using PBeta[of x p e2 e1' e2' e1] by fastforce . . .
+      subgoal for _ _ e1 e1' e2 e2' x using PBeta[of x p e2 e1' e2' e1] by fastforce . . .
 
 (* Also inferring equivariance from the general infrastructure: *)
 corollary rrename_pstep:
 assumes f: "bij f" "|supp f| <o |UNIV::var set|" 
 and r: "pstep e e'" 
 shows "pstep (rrename f e) (rrename f e')"
-using assms unfolding pstep_I using Pstep.I_equiv[of "(e,e')" f]
-unfolding Tperm_def isPerm_def by auto
+using assms unfolding pstep.alt_def using pstep.equiv[of "(e,e')" f]
+unfolding isPerm_def by auto
 
 
 end
